\documentclass[preview,varwidth=\maxdimen,border=10pt]{standalone}
\usepackage{ebproof,lplfitch}
\begin{document}
\begin{prooftree}
\infer{0}[\scriptsize Axiom]{p1, p4, p3, p2 &\vdash p1}
\infer{0}[\scriptsize Axiom]{p4, p3, p2 &\vdash p2, p1}
\infer{2}[\scriptsize $\liff$: Left]{p1 \liff p2, p4, p3, p2 &\vdash p1}
\infer{0}[\scriptsize Axiom]{p4, p3, p2 &\vdash p1 \liff p2, p3, p1}
\infer{2}[\scriptsize $\liff$: Left]{(p1 \liff p2) \liff p3, p4, p3, p2 &\vdash p1}
\infer{0}[\scriptsize Axiom]{p4, p3, p2 &\vdash (p1 \liff p2) \liff p3, p1, p4}
\infer{2}[\scriptsize $\liff$: Left]{((p1 \liff p2) \liff p3) \liff p4, p4, p3, p2 &\vdash p1}
\infer{0}[\scriptsize Axiom]{p1, p4, p3, p2 &\vdash p2}
\infer{0}[\scriptsize Axiom]{p1, p4, p3 &\vdash p2, p1}
\infer{2}[\scriptsize $\liff$: Left]{p1 \liff p2, p1, p4, p3 &\vdash p2}
\infer{0}[\scriptsize Axiom]{p1, p4, p3 &\vdash p1 \liff p2, p3, p2}
\infer{2}[\scriptsize $\liff$: Left]{(p1 \liff p2) \liff p3, p1, p4, p3 &\vdash p2}
\infer{0}[\scriptsize Axiom]{p1, p4, p3 &\vdash (p1 \liff p2) \liff p3, p2, p4}
\infer{2}[\scriptsize $\liff$: Left]{((p1 \liff p2) \liff p3) \liff p4, p1, p4, p3 &\vdash p2}
\infer{2}[\scriptsize $\liff$: Right]{((p1 \liff p2) \liff p3) \liff p4, p3, p4 &\vdash p2 \liff p1}
\infer{0}[\scriptsize Axiom]{p1 \liff p2, p1, p4, p3, p2 &\vdash p3}
\infer{0}[\scriptsize Axiom]{p1, p4, p2 &\vdash p3, p2}
\infer{0}[\scriptsize Axiom]{p1, p4, p2 &\vdash p3, p1}
\infer{2}[\scriptsize $\liff$: Right]{p1, p4, p2 &\vdash p1 \liff p2, p3}
\infer{2}[\scriptsize $\liff$: Left]{(p1 \liff p2) \liff p3, p1, p4, p2 &\vdash p3}
\infer{0}[\scriptsize Axiom]{p1, p4, p2 &\vdash (p1 \liff p2) \liff p3, p3, p4}
\infer{2}[\scriptsize $\liff$: Left]{((p1 \liff p2) \liff p3) \liff p4, p1, p4, p2 &\vdash p3}
\infer{0}[\scriptsize Axiom]{p1 \liff p2, p4, p3 &\vdash p3, p2, p1}
\infer{0}[\scriptsize Axiom]{p1, p4 &\vdash p3, p2, p1}
\infer{0}[\scriptsize Axiom]{p4, p2 &\vdash p3, p2, p1}
\infer{2}[\scriptsize $\liff$: Right]{p4 &\vdash p1 \liff p2, p3, p2, p1}
\infer{2}[\scriptsize $\liff$: Left]{(p1 \liff p2) \liff p3, p4 &\vdash p3, p2, p1}
\infer{0}[\scriptsize Axiom]{p4 &\vdash (p1 \liff p2) \liff p3, p3, p2, p1, p4}
\infer{2}[\scriptsize $\liff$: Left]{((p1 \liff p2) \liff p3) \liff p4, p4 &\vdash p3, p2, p1}
\infer{2}[\scriptsize $\liff$: Left]{((p1 \liff p2) \liff p3) \liff p4, p2 \liff p1, p4 &\vdash p3}
\infer{2}[\scriptsize $\liff$: Right]{((p1 \liff p2) \liff p3) \liff p4, p4 &\vdash p3 \liff (p2 \liff p1)}
\infer{0}[\scriptsize Axiom]{(p1 \liff p2) \liff p3, p1, p4, p3, p2 &\vdash p4}
\infer{0}[\scriptsize Axiom]{p1 \liff p2, p1, p3, p2 &\vdash p3, p4}
\infer{0}[\scriptsize Axiom]{p1, p3, p2 &\vdash p2, p4}
\infer{0}[\scriptsize Axiom]{p1, p3, p2 &\vdash p1, p4}
\infer{2}[\scriptsize $\liff$: Right]{p1, p3, p2 &\vdash p1 \liff p2, p4}
\infer{2}[\scriptsize $\liff$: Right]{p1, p3, p2 &\vdash (p1 \liff p2) \liff p3, p4}
\infer{2}[\scriptsize $\liff$: Left]{((p1 \liff p2) \liff p3) \liff p4, p1, p3, p2 &\vdash p4}
\infer{0}[\scriptsize Axiom]{(p1 \liff p2) \liff p3, p3, p4 &\vdash p2, p1, p4}
\infer{0}[\scriptsize Axiom]{p1 \liff p2, p3 &\vdash p3, p2, p1, p4}
\infer{0}[\scriptsize Axiom]{p1, p3 &\vdash p2, p1, p4}
\infer{0}[\scriptsize Axiom]{p3, p2 &\vdash p2, p1, p4}
\infer{2}[\scriptsize $\liff$: Right]{p3 &\vdash p1 \liff p2, p2, p1, p4}
\infer{2}[\scriptsize $\liff$: Right]{p3 &\vdash (p1 \liff p2) \liff p3, p2, p1, p4}
\infer{2}[\scriptsize $\liff$: Left]{((p1 \liff p2) \liff p3) \liff p4, p3 &\vdash p2, p1, p4}
\infer{2}[\scriptsize $\liff$: Left]{((p1 \liff p2) \liff p3) \liff p4, p2 \liff p1, p3 &\vdash p4}
\infer{0}[\scriptsize Axiom]{(p1 \liff p2) \liff p3, p4, p2 &\vdash p3, p1, p4}
\infer{0}[\scriptsize Axiom]{p1, p2 &\vdash p3, p1, p4}
\infer{0}[\scriptsize Axiom]{p2 &\vdash p3, p2, p1, p4}
\infer{2}[\scriptsize $\liff$: Left]{p1 \liff p2, p2 &\vdash p3, p1, p4}
\infer{0}[\scriptsize Axiom]{p3, p2 &\vdash p1 \liff p2, p3, p1, p4}
\infer{2}[\scriptsize $\liff$: Right]{p2 &\vdash (p1 \liff p2) \liff p3, p3, p1, p4}
\infer{2}[\scriptsize $\liff$: Left]{((p1 \liff p2) \liff p3) \liff p4, p2 &\vdash p3, p1, p4}
\infer{0}[\scriptsize Axiom]{(p1 \liff p2) \liff p3, p1, p4 &\vdash p3, p2, p4}
\infer{0}[\scriptsize Axiom]{p1, p2 &\vdash p3, p2, p4}
\infer{0}[\scriptsize Axiom]{p1 &\vdash p3, p2, p1, p4}
\infer{2}[\scriptsize $\liff$: Left]{p1 \liff p2, p1 &\vdash p3, p2, p4}
\infer{0}[\scriptsize Axiom]{p1, p3 &\vdash p1 \liff p2, p3, p2, p4}
\infer{2}[\scriptsize $\liff$: Right]{p1 &\vdash (p1 \liff p2) \liff p3, p3, p2, p4}
\infer{2}[\scriptsize $\liff$: Left]{((p1 \liff p2) \liff p3) \liff p4, p1 &\vdash p3, p2, p4}
\infer{2}[\scriptsize $\liff$: Right]{((p1 \liff p2) \liff p3) \liff p4 &\vdash p2 \liff p1, p3, p4}
\infer{2}[\scriptsize $\liff$: Left]{((p1 \liff p2) \liff p3) \liff p4, p3 \liff (p2 \liff p1) &\vdash p4}
\infer{2}[\scriptsize $\liff$: Right]{((p1 \liff p2) \liff p3) \liff p4 &\vdash p4 \liff (p3 \liff (p2 \liff p1))}
\infer{0}[\scriptsize Axiom]{p3 \liff (p2 \liff p1), p1, p4, p3, p2 &\vdash p4}
\infer{0}[\scriptsize Axiom]{p1, p3, p2 &\vdash p1, p4}
\infer{0}[\scriptsize Axiom]{p1, p3, p2 &\vdash p2, p4}
\infer{2}[\scriptsize $\liff$: Right]{p1, p3, p2 &\vdash p2 \liff p1, p4}
\infer{0}[\scriptsize Axiom]{p2 \liff p1, p1, p3, p2 &\vdash p3, p4}
\infer{2}[\scriptsize $\liff$: Right]{p1, p3, p2 &\vdash p3 \liff (p2 \liff p1), p4}
\infer{2}[\scriptsize $\liff$: Left]{p4 \liff (p3 \liff (p2 \liff p1)), p1, p3, p2 &\vdash p4}
\infer{0}[\scriptsize Axiom]{p3 \liff (p2 \liff p1), p3, p4 &\vdash p2, p1, p4}
\infer{0}[\scriptsize Axiom]{p3, p2 &\vdash p2, p1, p4}
\infer{0}[\scriptsize Axiom]{p1, p3 &\vdash p2, p1, p4}
\infer{2}[\scriptsize $\liff$: Right]{p3 &\vdash p2 \liff p1, p2, p1, p4}
\infer{0}[\scriptsize Axiom]{p2 \liff p1, p3 &\vdash p3, p2, p1, p4}
\infer{2}[\scriptsize $\liff$: Right]{p3 &\vdash p3 \liff (p2 \liff p1), p2, p1, p4}
\infer{2}[\scriptsize $\liff$: Left]{p4 \liff (p3 \liff (p2 \liff p1)), p3 &\vdash p2, p1, p4}
\infer{2}[\scriptsize $\liff$: Left]{p4 \liff (p3 \liff (p2 \liff p1)), p1 \liff p2, p3 &\vdash p4}
\infer{0}[\scriptsize Axiom]{p3 \liff (p2 \liff p1), p1, p4 &\vdash p3, p2, p4}
\infer{0}[\scriptsize Axiom]{p1, p3 &\vdash p2 \liff p1, p3, p2, p4}
\infer{0}[\scriptsize Axiom]{p1, p2 &\vdash p3, p2, p4}
\infer{0}[\scriptsize Axiom]{p1 &\vdash p3, p2, p1, p4}
\infer{2}[\scriptsize $\liff$: Left]{p2 \liff p1, p1 &\vdash p3, p2, p4}
\infer{2}[\scriptsize $\liff$: Right]{p1 &\vdash p3 \liff (p2 \liff p1), p3, p2, p4}
\infer{2}[\scriptsize $\liff$: Left]{p4 \liff (p3 \liff (p2 \liff p1)), p1 &\vdash p3, p2, p4}
\infer{0}[\scriptsize Axiom]{p3 \liff (p2 \liff p1), p4, p2 &\vdash p3, p1, p4}
\infer{0}[\scriptsize Axiom]{p3, p2 &\vdash p2 \liff p1, p3, p1, p4}
\infer{0}[\scriptsize Axiom]{p1, p2 &\vdash p3, p1, p4}
\infer{0}[\scriptsize Axiom]{p2 &\vdash p3, p2, p1, p4}
\infer{2}[\scriptsize $\liff$: Left]{p2 \liff p1, p2 &\vdash p3, p1, p4}
\infer{2}[\scriptsize $\liff$: Right]{p2 &\vdash p3 \liff (p2 \liff p1), p3, p1, p4}
\infer{2}[\scriptsize $\liff$: Left]{p4 \liff (p3 \liff (p2 \liff p1)), p2 &\vdash p3, p1, p4}
\infer{2}[\scriptsize $\liff$: Right]{p4 \liff (p3 \liff (p2 \liff p1)) &\vdash p1 \liff p2, p3, p4}
\infer{2}[\scriptsize $\liff$: Left]{p4 \liff (p3 \liff (p2 \liff p1)), (p1 \liff p2) \liff p3 &\vdash p4}
\infer{0}[\scriptsize Axiom]{p2 \liff p1, p1, p4, p3, p2 &\vdash p3}
\infer{0}[\scriptsize Axiom]{p1, p4, p2 &\vdash p3, p1}
\infer{0}[\scriptsize Axiom]{p1, p4, p2 &\vdash p3, p2}
\infer{2}[\scriptsize $\liff$: Right]{p1, p4, p2 &\vdash p2 \liff p1, p3}
\infer{2}[\scriptsize $\liff$: Left]{p3 \liff (p2 \liff p1), p1, p4, p2 &\vdash p3}
\infer{0}[\scriptsize Axiom]{p1, p4, p2 &\vdash p3 \liff (p2 \liff p1), p3, p4}
\infer{2}[\scriptsize $\liff$: Left]{p4 \liff (p3 \liff (p2 \liff p1)), p1, p4, p2 &\vdash p3}
\infer{0}[\scriptsize Axiom]{p2 \liff p1, p4, p3 &\vdash p3, p2, p1}
\infer{0}[\scriptsize Axiom]{p4, p2 &\vdash p3, p2, p1}
\infer{0}[\scriptsize Axiom]{p1, p4 &\vdash p3, p2, p1}
\infer{2}[\scriptsize $\liff$: Right]{p4 &\vdash p2 \liff p1, p3, p2, p1}
\infer{2}[\scriptsize $\liff$: Left]{p3 \liff (p2 \liff p1), p4 &\vdash p3, p2, p1}
\infer{0}[\scriptsize Axiom]{p4 &\vdash p3 \liff (p2 \liff p1), p3, p2, p1, p4}
\infer{2}[\scriptsize $\liff$: Left]{p4 \liff (p3 \liff (p2 \liff p1)), p4 &\vdash p3, p2, p1}
\infer{2}[\scriptsize $\liff$: Left]{p4 \liff (p3 \liff (p2 \liff p1)), p1 \liff p2, p4 &\vdash p3}
\infer{0}[\scriptsize Axiom]{p1, p4, p3, p2 &\vdash p2}
\infer{0}[\scriptsize Axiom]{p1, p4, p3 &\vdash p2, p1}
\infer{2}[\scriptsize $\liff$: Left]{p2 \liff p1, p1, p4, p3 &\vdash p2}
\infer{0}[\scriptsize Axiom]{p1, p4, p3 &\vdash p2 \liff p1, p3, p2}
\infer{2}[\scriptsize $\liff$: Left]{p3 \liff (p2 \liff p1), p1, p4, p3 &\vdash p2}
\infer{0}[\scriptsize Axiom]{p1, p4, p3 &\vdash p3 \liff (p2 \liff p1), p2, p4}
\infer{2}[\scriptsize $\liff$: Left]{p4 \liff (p3 \liff (p2 \liff p1)), p1, p4, p3 &\vdash p2}
\infer{0}[\scriptsize Axiom]{p1, p4, p3, p2 &\vdash p1}
\infer{0}[\scriptsize Axiom]{p4, p3, p2 &\vdash p2, p1}
\infer{2}[\scriptsize $\liff$: Left]{p2 \liff p1, p4, p3, p2 &\vdash p1}
\infer{0}[\scriptsize Axiom]{p4, p3, p2 &\vdash p2 \liff p1, p3, p1}
\infer{2}[\scriptsize $\liff$: Left]{p3 \liff (p2 \liff p1), p4, p3, p2 &\vdash p1}
\infer{0}[\scriptsize Axiom]{p4, p3, p2 &\vdash p3 \liff (p2 \liff p1), p1, p4}
\infer{2}[\scriptsize $\liff$: Left]{p4 \liff (p3 \liff (p2 \liff p1)), p4, p3, p2 &\vdash p1}
\infer{2}[\scriptsize $\liff$: Right]{p4 \liff (p3 \liff (p2 \liff p1)), p3, p4 &\vdash p1 \liff p2}
\infer{2}[\scriptsize $\liff$: Right]{p4 \liff (p3 \liff (p2 \liff p1)), p4 &\vdash (p1 \liff p2) \liff p3}
\infer{2}[\scriptsize $\liff$: Right]{p4 \liff (p3 \liff (p2 \liff p1)) &\vdash ((p1 \liff p2) \liff p3) \liff p4}
\infer{2}[\scriptsize $\liff$: Right]{ &\vdash (((p1 \liff p2) \liff p3) \liff p4) \liff (p4 \liff (p3 \liff (p2 \liff p1)))}
\end{prooftree}
\end{document}
